src/Init/Data/Array/TakeDrop.lean
@@ -12,7 +12,7 @@ namespace Array
 theorem exists_of_uset (self : Array α) (i d h) :
     ∃ l₁ l₂, self.toList = l₁ ++ self[i] :: l₂ ∧ List.length l₁ = i.toNat ∧
       (self.uset i d h).toList = l₁ ++ d :: l₂ := by
-  simpa only [ugetElem_eq_getElem, getElem_eq_getElem_toList, uset, toList_set] using
+  simpa only [ugetElem_eq_getElem, ← getElem_toList, uset, toList_set] using
     List.exists_of_set _
 
 end Array
